theories/Dot/operational.v
@@ -8,81 +8,23 @@ From iris.program_logic Require Import weakestpre.
 From D Require Import tactics.
 From D.Dot Require Export dotsyn.
 
+(* gen_iheap *)
+From D Require Export saved_interp.
+
 Class dotG Σ := DotG {
   dotG_invG : invG Σ;
-  dotG_savior :> savedAnythingG Σ (vls -c> vl -c> ▶ ∙)
+  dotG_savior :> savedInterpG Σ vls vl
 }.
 
 Class dotPreG Σ := DotPreG {
   dotPreG_invG : invPreG Σ;
-  dotPreG_savior :> savedAnythingG Σ (vls -c> vl -c> ▶ ∙)
+  dotPreG_savior :> savedInterpG Σ vls vl
 }.
 
-Definition dotΣ := #[invΣ; savedAnythingΣ (vls -c> vl -c> ▶ ∙)].
+Definition dotΣ := #[invΣ; savedInterpΣ vls vl].
 
 Instance subG_dotΣ {Σ} : subG dotΣ Σ → dotPreG Σ.
 Proof. solve_inG. Qed.
-
-(** saved interpretations *)
-
-Section saved_interp.
-  Context `{!dotG Σ}.
-
-  Definition saved_interp_own (γ : gname) (Φ : vls → vl → iProp Σ) :=
-    saved_anything_own
-      (F := vls -c> vl -c> ▶ ∙) γ (λ vs v, CofeMor Next (Φ vs v)).
-
-Instance saved_interp_own_contractive γ :
-  Contractive (saved_interp_own γ : (vls -c> vl -c> iProp Σ) → iProp Σ).
-Proof.
-  intros n X Y HXY.
-  rewrite /saved_interp_own /saved_anything_own /=.
-  f_equiv. apply to_agree_ne; f_equiv.
-  intros x y.
-  apply Next_contractive.
-  destruct n; simpl in *; auto.
-  apply HXY.
-Qed.
-
-Lemma saved_interp_alloc_strong (G : gset gname) (Φ : vls → vl → iProp Σ) :
-  (|==> ∃ γ, ⌜γ ∉ G⌝ ∧ saved_interp_own γ Φ)%I.
-Proof. iApply saved_anything_alloc_strong. Qed.
-
-Lemma saved_interp_alloc (Φ : vls → vl → iProp Σ) :
-  (|==> ∃ γ, saved_interp_own γ Φ)%I.
-Proof. iApply saved_anything_alloc. Qed.
-
-Lemma saved_interp_agree γ Φ Ψ vs v :
-  saved_interp_own γ Φ -∗ saved_interp_own γ Ψ -∗ ▷ (Φ vs v ≡ Ψ vs v).
-Proof.
-  unfold saved_pred_own. iIntros "#HΦ #HΨ /=". iApply bi.later_equivI.
-  iDestruct (saved_anything_agree with "HΦ HΨ") as "Heq".
-  rewrite bi.ofe_fun_equivI; iSpecialize ("Heq" $! vs).
-  by rewrite bi.ofe_fun_equivI; iSpecialize ("Heq" $! v); simpl.
-Qed.
-
-Lemma saved_interp_agree_eta γ Φ Ψ vs v :
-  saved_interp_own γ (λ (vs : vls) (v : vl), (Φ vs) v) -∗
-  saved_interp_own γ (λ (vs : vls) (v : vl), (Ψ vs) v) -∗
-  ▷ (Φ vs v ≡ Ψ vs v).
-Proof.
-  iIntros "#H1 #H2".  
-  repeat change (fun x => ?h x) with h.
-  by iApply saved_interp_agree.
-Qed.
-
-Lemma saved_interp_impl γ Φ Ψ vs v :
-  saved_interp_own γ Φ -∗ saved_interp_own γ Ψ -∗ □ (▷ Φ vs v -∗ ▷ Ψ vs v).
-Proof.
-  unfold saved_pred_own. iIntros "#HΦ #HΨ /= !# H1".
-  iDestruct (saved_anything_agree with "HΦ HΨ") as "Heq".
-  rewrite bi.ofe_fun_equivI; iSpecialize ("Heq" $! vs).
-  rewrite bi.ofe_fun_equivI; iSpecialize ("Heq" $! v); simpl.
-  rewrite bi.later_equivI.
-  by iNext; iRewrite -"Heq".
-Qed.
-
-End saved_interp.
 
 Implicit Types
          (T: ty) (v: vl) (t e: tm) (d: dm) (ds: dms) (vs: vls)
@@ -337,8 +279,6 @@ Section Sec.
 
   Canonical Structure listVlC := leibnizC (list vl).
 End Sec.
-
-Notation "g ⤇ p" := (saved_interp_own g p) (at level 20).
 
 (* For abstracting synToSem. *)
 Class dotInterpG Σ := DotInterpG {
