theories/saved_interp.v
@@ -1,0 +1,74 @@
+From iris.algebra Require Import ofe agree.
+From iris.proofmode Require Import tactics.
+From iris.base_logic Require Import lib.iprop (* For gname *)
+     lib.saved_prop.
+From iris.program_logic Require Import weakestpre.
+
+From D Require Import tactics.
+
+(** saved interpretations *)
+
+Notation savedInterpG Σ A B := (savedAnythingG Σ (A -c> B -c> ▶ ∙)).
+Notation savedInterpΣ A B := (savedAnythingΣ (A -c> B -c> ▶ ∙)).
+Section saved_interp.
+  Context {vls vl: Type}.
+  Context `{!savedInterpG Σ vls vl}.
+  (* Context `{!savedAnythingG Σ (vls -c> vl -c> ▶ ∙)}. *)
+
+  Definition saved_interp_own (γ : gname) (Φ : vls → vl → iProp Σ) :=
+    saved_anything_own
+      (F := vls -c> vl -c> ▶ ∙) γ (λ vs v, CofeMor Next (Φ vs v)).
+
+  Instance saved_interp_own_contractive γ :
+    Contractive (saved_interp_own γ : (vls -c> vl -c> iProp Σ) → iProp Σ).
+  Proof.
+    intros n X Y HXY.
+    rewrite /saved_interp_own /saved_anything_own /=.
+    f_equiv. apply to_agree_ne; f_equiv.
+    intros x y.
+    apply Next_contractive.
+    destruct n; simpl in *; auto.
+    apply HXY.
+  Qed.
+
+  Lemma saved_interp_alloc_strong (G : gset gname) (Φ : vls → vl → iProp Σ) :
+    (|==> ∃ γ, ⌜γ ∉ G⌝ ∧ saved_interp_own γ Φ)%I.
+  Proof. iApply saved_anything_alloc_strong. Qed.
+
+  Lemma saved_interp_alloc (Φ : vls → vl → iProp Σ) :
+    (|==> ∃ γ, saved_interp_own γ Φ)%I.
+  Proof. iApply saved_anything_alloc. Qed.
+
+  Lemma saved_interp_agree γ Φ Ψ vs v :
+    saved_interp_own γ Φ -∗ saved_interp_own γ Ψ -∗ ▷ (Φ vs v ≡ Ψ vs v).
+  Proof.
+    unfold saved_pred_own. iIntros "#HΦ #HΨ /=". iApply bi.later_equivI.
+    iDestruct (saved_anything_agree with "HΦ HΨ") as "Heq".
+    rewrite bi.ofe_fun_equivI; iSpecialize ("Heq" $! vs).
+    by rewrite bi.ofe_fun_equivI; iSpecialize ("Heq" $! v); simpl.
+  Qed.
+
+  Lemma saved_interp_agree_eta γ Φ Ψ vs v :
+    saved_interp_own γ (λ (vs : vls) (v : vl), (Φ vs) v) -∗
+    saved_interp_own γ (λ (vs : vls) (v : vl), (Ψ vs) v) -∗
+    ▷ (Φ vs v ≡ Ψ vs v).
+  Proof.
+    iIntros "#H1 #H2".
+    repeat change (fun x => ?h x) with h.
+    by iApply saved_interp_agree.
+  Qed.
+
+  Lemma saved_interp_impl γ Φ Ψ vs v :
+    saved_interp_own γ Φ -∗ saved_interp_own γ Ψ -∗ □ (▷ Φ vs v -∗ ▷ Ψ vs v).
+  Proof.
+    unfold saved_pred_own. iIntros "#HΦ #HΨ /= !# H1".
+    iDestruct (saved_anything_agree with "HΦ HΨ") as "Heq".
+    rewrite bi.ofe_fun_equivI; iSpecialize ("Heq" $! vs).
+    rewrite bi.ofe_fun_equivI; iSpecialize ("Heq" $! v); simpl.
+    rewrite bi.later_equivI.
+    by iNext; iRewrite -"Heq".
+  Qed.
+
+End saved_interp.
+
+Notation "g ⤇ p" := (saved_interp_own g p) (at level 20).
